Henret/Proofs.lean
@@ -8,6 +8,7 @@ import Henret.Proofs.Invariants
 import Henret.Proofs.InvariantsPreservation
 import Henret.Proofs.ResourceReachable
 import Henret.Proofs.ResourceBranch
+import Henret.Proofs.Policy
 import Henret.Proofs.Parenthood
 import Henret.Proofs.Occurrence
 import Henret.Proofs.Supervision
